vst/verif_treeclock.v
@@ -1,6 +1,6 @@
 Require Import VST.floyd.proofauto.
-Require Import distributedclocks.vst.treeclock_clight.
 Require Import distributedclocks.clocks.treeclock.
+From distributedclocks.vst Require Import treeclock_clight util_vst.
 
 #[export] Instance CompSpecs : compspecs. make_compspecs prog. Defined.
 Definition Vprog : varspecs. mk_varspecs prog. Defined.
@@ -16,32 +16,6 @@ TODO change tid to be Z, and use Znth? this may be troublesome since id should >
 Definition t_struct_clock := Tstruct _Clock noattr.
 Definition t_struct_node := Tstruct _Node noattr.
 Definition t_struct_treeclock := Tstruct _TreeClock noattr.
-
-Definition short_max_signed := two_power_nat 15 - 1.
-
-(* TODO why so tedious *)
-Fact Zpower_nat_gt_0 b n : b > 0 -> 0 < Zpower_nat b n.
-Proof. induction n; intros; simpl; try nia. Qed.
-
-Fact short_max_signed_le_int_max_signed : short_max_signed <= Int.max_signed.
-Proof. 
-  unfold Int.max_signed, Int.half_modulus, Int.modulus, short_max_signed, Int.wordsize, Wordsize_32.wordsize.
-  unfold two_power_nat. 
-  rewrite -> ! shift_nat_correct, -> ! Z.mul_1_r.
-  rewrite -> Zaux.Zpower_nat_S with (e:=31%nat), -> Z.mul_comm, -> Z_div_mult; try lia.
-  replace 31%nat with (16+15)%nat by lia.
-  rewrite -> Zpower_nat_is_exp.
-  pose proof (Zpower_nat_gt_0 2%Z 15) as H. removehead H; try lia.
-  pose proof (Zpower_nat_gt_0 2%Z 16) as H0. removehead H0; try lia.
-  nia.
-Qed.
-
-Fact short_max_signed_gt_0 : 0 < short_max_signed.
-Proof. 
-  unfold short_max_signed, two_power_nat. 
-  rewrite -> shift_nat_correct, -> Zaux.Zpower_nat_S.
-  pose proof (Zpower_nat_gt_0 2%Z 14) as H. removehead H; try lia.
-Qed.
 
 Definition is_pos_tint z : Prop := 0 <= z <= Int.max_signed.
 (* planned not to use *)
@@ -74,41 +48,61 @@ Definition node_rep (lch rch par headch : Z) (p : val) : mpred :=
 #[export] Instance nat_EqDec : EqDec nat.
 Proof. constructor. apply Nat.eq_dec. Qed.
 
+(* using Z as the thread type is difficult, since we cannot guarantee the positiveness ... *)
+(*
 #[export] Instance Z_EqDec : EqDec Z.
 Proof. constructor. apply Z.eq_dec. Qed.
+*)
+
+(* here, there is a choice between nth_error and Znth. 
+  for now, the choice is to make more use of nth_error, since there is no counterpart 
+  like Znth_error;
+  but for the array part, we will switch to Znth since Znth is more commonly used there
+
+  for length, we try consistently using Zlength
+*)
 
 Definition is_tc_clockarray_proj (l : list (reptype t_struct_clock)) (tc : treeclock) : Prop :=
   Foralltc (fun t => nth_error l (tc_roottid t) = 
     Some (clock_payload (Z.of_nat (tc_rootclk t)) (Z.of_nat (tc_rootaclk t)))) tc.
 
 Definition clockarray_emptypart (l : list (reptype t_struct_clock)) (tc : treeclock) : Prop :=
-  forall n, tc_getnode n tc = None -> nth_error l n = Some (clock_payload 0%Z 0%Z).
+  forall n np, tc_getnode n tc = None -> nth_error l n = Some np -> 
+    np = clock_payload 0%Z 0%Z.
 
 (* TODO could also be per-field description so that there will be only one branch *)
 
-Definition is_tc_nodearray_proj_chnaux (par headch : nat) (l : list (reptype t_struct_node)) :
-  nat -> list treeclock -> Prop := 
+(* typically requires that default_nodefield <= 0 *)
+Definition default_nodefield := (-1)%Z.
+
+Definition default_nodestruct := node_payload default_nodefield default_nodefield default_nodefield default_nodefield.
+
+Definition tc_headch_Z (tc : @treeclock nat) : Z := 
+  match tc_rootchn tc with nil => (-1)%Z | ch :: _ => Z.of_nat (tc_roottid ch) end.
+
+Definition is_tc_nodearray_proj_chnaux (par : nat) (l : list (reptype t_struct_node)) :
+  forall (lch : Z) (chn : list treeclock), Prop := 
   fix aux lch chn {struct chn} : Prop := 
   match chn with
-  | nil => True (* hopefully will not enter this *)
+  | nil => True
   | ch :: chn' => 
-    let tmp := aux (tc_roottid ch) chn' in 
+    (* let tmp := aux (Z.of_nat (tc_roottid ch)) chn' in  *)
+    nth_error l (tc_roottid ch) = 
+    Some (node_payload lch 
+      (match chn' with nil => default_nodefield | ch' :: _ => (Z.of_nat (tc_roottid ch')) end) 
+      (Z.of_nat par) (tc_headch_Z ch)) /\
+    aux (Z.of_nat (tc_roottid ch)) chn'
+    (*
     match chn' with
     | nil =>
       nth_error l (tc_roottid ch) = 
-      Some (node_payload (Z.of_nat lch) 0%Z (Z.of_nat par) (Z.of_nat headch))
+      Some (node_payload lch default_nodefield (Z.of_nat par) (tc_headch_Z ch))
     | ch' :: _ =>
       nth_error l (tc_roottid ch) = 
-      Some (node_payload (Z.of_nat lch) (Z.of_nat (tc_roottid ch')) (Z.of_nat par) (Z.of_nat headch))
+      Some (node_payload lch (Z.of_nat (tc_roottid ch')) (Z.of_nat par) (tc_headch_Z ch))
       /\ tmp
     end
-  end.
-
-Definition is_tc_nodearray_proj_aux (l : list (reptype t_struct_node)) (tc : @treeclock nat): Prop :=
-  let: Node _ chn := tc in 
-  match chn with
-  | nil => True
-  | ch :: _ => is_tc_nodearray_proj_chnaux (tc_roottid tc) (tc_roottid ch) l 0%nat chn
+    *)
   end.
 
 (*
@@ -128,11 +122,31 @@ Definition is_tc_nodearray_proj_aux (par headch : nat) (l : list (reptype t_stru
   end. 
 *)
 
+Definition is_tc_nodearray_proj_aux (l : list (reptype t_struct_node)) (tc : @treeclock nat): Prop :=
+  is_tc_nodearray_proj_chnaux (tc_roottid tc) l default_nodefield (tc_rootchn tc).
+  (*
+  let: Node _ chn := tc in 
+  match chn with
+  | nil => True
+  | ch :: _ => is_tc_nodearray_proj_chnaux (tc_roottid tc) l default_nodefield chn
+  end.
+  *)
+
+Global Arguments is_tc_nodearray_proj_aux _ _/.
+
+Definition is_tc_nodearray_proj_root (l : list (reptype t_struct_node)) (tc : @treeclock nat): Prop :=
+  nth_error l (tc_roottid tc) = 
+  Some (node_payload default_nodefield default_nodefield default_nodefield (tc_headch_Z tc)).
+
 Definition is_tc_nodearray_proj (l : list (reptype t_struct_node)) (tc : @treeclock nat) : Prop :=
   Foralltc (is_tc_nodearray_proj_aux l) tc.
 
+(* for the whole tree *)
+Definition is_tc_nodearray_proj_full (l : list (reptype t_struct_node)) (tc : @treeclock nat) : Prop :=
+  is_tc_nodearray_proj_root l tc /\ is_tc_nodearray_proj l tc.
+
 Definition nodearray_emptypart (l : list (reptype t_struct_node)) (tc : @treeclock nat) : Prop :=
-  forall n, tc_getnode n tc = None -> nth_error l n = Some (node_payload 0%Z 0%Z 0%Z 0%Z).
+  forall n np, tc_getnode n tc = None -> nth_error l n = Some np -> np = default_nodestruct.
 
 Definition treeclock_payload (dim rootid : Z) (clockarr nodearr : val) 
   (stk : val) (top : Z) : reptype t_struct_treeclock :=
@@ -166,6 +180,164 @@ Definition treeclock_rep (dim : Z) (tc : @treeclock nat) (plclk plnode : val)
   data_at Tsh (tarray t_struct_node dim) lnode plnode *
   (* data_at Tsh (tarray tshort dim) lstk plstk. *)
   data_at Tsh (tarray tint dim) lstk plstk.
+
+(* simple bounded properties *)
+(* TODO should I use Z.< instead? *)
+
+Fact is_tc_nodearray_proj_chnaux_tid_bounded lnode par lch chn (Hproj : is_tc_nodearray_proj_chnaux par lnode lch chn) :
+  Forall (fun tc' => Z.of_nat (tc_roottid tc') < Zlength lnode) chn.
+Proof.
+  revert lnode lch Hproj.
+  induction chn as [ | ch chn IH ]; intros; constructor; simpl in Hproj.
+  - now apply proj1, nth_error_some_inrange_Z in Hproj.
+  - eapply IH. apply (proj2 Hproj).
+Qed.
+
+(*
+Fact is_tc_nodearray_proj_aux_tid_bounded lnode tc (Hproj : is_tc_nodearray_proj_aux lnode tc) :
+  Forall (fun tc' => Z.of_nat (tc_roottid tc') < Zlength lnode) (tc_rootchn tc).
+Proof.
+  destruct tc as [(u, clk, aclk) chn].
+  now apply is_tc_nodearray_proj_chnaux_tid_bounded in Hproj.
+Qed.
+*)
+
+Fact is_tc_nodearray_proj_tid_bounded lnode tc (Hproj : is_tc_nodearray_proj lnode tc)
+  (HH : Z.of_nat (tc_roottid tc) < Zlength lnode) :
+  Foralltc (fun tc' => Z.of_nat (tc_roottid tc') < Zlength lnode) tc.
+Proof.
+  revert lnode Hproj HH.
+  induction tc as [(u, clk, aclk) chn IH] using treeclock_ind_2; intros.
+  simpl in HH.
+  apply Foralltc_cons_iff in Hproj. destruct Hproj as (Hchn & Hproj). 
+  constructor; simpl; auto.
+  apply is_tc_nodearray_proj_chnaux_tid_bounded in Hchn.
+  rewrite -> Forall_forall in IH, Hproj, Hchn |- *.
+  intros ch Hin. specialize (Hproj _ Hin). specialize (Hchn _ Hin). apply IH; auto.
+Qed.
+
+Definition node_struct_regular dim np : Prop :=
+  exists z1 z2 z3 z4, 
+    np = node_payload z1 z2 z3 z4 /\
+    default_nodefield <= z1 < dim /\
+    default_nodefield <= z2 < dim /\
+    default_nodefield <= z3 < dim /\
+    default_nodefield <= z4 < dim.
+
+Fact is_tc_nodearray_proj_chnaux_regular lnode par lch chn (Hproj : is_tc_nodearray_proj_chnaux par lnode lch chn)
+  (* dim (Hlen : Zlength lnode = dim)  *)
+  (Hu : Z.of_nat par < Zlength lnode) (Hlch : default_nodefield <= lch < Zlength lnode)
+  (Hchn : Forall (fun ch => default_nodefield <= tc_headch_Z ch < Zlength lnode) chn) :
+  Forall (fun tc' => node_struct_regular (Zlength lnode) (Znth (Z.of_nat (tc_roottid tc')) lnode)) chn.
+Proof.
+  revert lch lnode Hu Hproj Hlch Hchn. 
+  induction chn as [ | ch chn IH ]; intros; constructor; simpl in Hproj.
+  - hnf.
+    match type of Hproj with _ = Some (node_payload ?z1 ?z2 ?z3 ?z4) /\ _ => 
+      exists z1, z2, z3, z4 end.
+    split. 1: now apply proj1, nth_error_Znth_result in Hproj.
+    split; auto. split. 2: split; [ unfold default_nodefield; lia | now inversion Hchn ].
+    destruct chn. 
+    2: apply proj2, is_tc_nodearray_proj_chnaux_tid_bounded in Hproj.
+    2: rewrite -> Forall_cons_iff in Hproj; destruct Hproj as (Hproj & _).
+    all: unfold default_nodefield; lia.
+  - destruct Hproj as (Htmp & Hproj). apply nth_error_some_inrange_Z in Htmp.
+    inversion_clear Hchn.
+    apply IH with (lch:=(Z.of_nat (tc_roottid ch))); auto; unfold default_nodefield; try lia; try tauto.
+Qed. 
+
+(*
+Fact is_tc_nodearray_proj_aux_regular lnode tc (Hproj : is_tc_nodearray_proj_aux lnode tc)
+  dim (Hlen : Zlength lnode = dim)
+  (Hu : Z.of_nat (tc_roottid tc) < dim)
+  (Hchn : Forall (fun ch => default_nodefield <= tc_headch_Z ch < dim) (tc_rootchn tc)) :
+  Forall (fun tc' => node_struct_regular dim (Znth (Z.of_nat (tc_roottid tc')) lnode)) (tc_rootchn tc).
+Proof.
+  destruct tc as [(u, clk, aclk) chn].
+  simpl in Hu, Hproj, Hchn |- *.
+  destruct chn. 1: constructor.
+  eapply is_tc_nodearray_proj_chnaux_regular; eauto.
+  unfold default_nodefield. lia.
+Qed.
+*)
+
+(* TODO may need revise *)
+
+Fact is_tc_nodearray_proj_headch_inrange lnode tc (Hproj : is_tc_nodearray_proj lnode tc) :
+  default_nodefield <= tc_headch_Z tc < Zlength lnode.
+Proof.
+  unfold default_nodefield, tc_headch_Z.
+  pose proof (Zlength_nonneg lnode).
+  destruct tc as [ ? [ | ] ]; simpl; try lia.
+  apply Foralltc_self in Hproj. 
+  apply is_tc_nodearray_proj_chnaux_tid_bounded in Hproj; auto.
+  inversion_clear Hproj. lia.
+Qed.
+
+Fact is_tc_nodearray_proj_regular lnode tc (Hproj : is_tc_nodearray_proj lnode tc)
+  (* dim (Hlen : Zlength lnode = dim)  *)
+  (Hu : Z.of_nat (tc_roottid tc) < (Zlength lnode))
+  (HH : node_struct_regular (Zlength lnode) (Znth (Z.of_nat (tc_roottid tc)) lnode)) :
+  Foralltc (fun tc' => node_struct_regular (Zlength lnode) (Znth (Z.of_nat (tc_roottid tc')) lnode)) tc.
+Proof.
+  revert lnode Hproj Hu HH.
+  induction tc as [(u, clk, aclk) chn IH] using treeclock_ind_2; intros.
+  simpl in HH, Hu.
+  apply Foralltc_cons_iff in Hproj. destruct Hproj as (Hchn & Hproj). 
+  constructor; simpl; auto.
+  simpl in Hchn.
+  pose proof Hchn as Hchn'. apply is_tc_nodearray_proj_chnaux_tid_bounded in Hchn'.
+  apply is_tc_nodearray_proj_chnaux_regular in Hchn; simpl; auto.
+  2: unfold default_nodefield; lia.
+  2:{
+    rewrite -> Forall_forall in Hproj, Hchn' |- *. 
+    intros ch Hin. specialize (Hproj _ Hin). specialize (Hchn' _ Hin).
+    now apply is_tc_nodearray_proj_headch_inrange in Hproj.
+  }
+  rewrite -> Forall_forall in IH, Hproj, Hchn, Hchn' |- *.
+  intros ch Hin. specialize (Hproj _ Hin). specialize (Hchn _ Hin). specialize (Hchn' _ Hin). 
+  apply IH; auto.
+Qed.
+
+Fact is_tc_nodearray_proj_full_regular lnode tc (Hproj : is_tc_nodearray_proj_full lnode tc) :
+  (* dim (Hlen : Zlength lnode = dim)  *)
+  (* (Hu : Z.of_nat (tc_roottid tc) < (Zlength lnode))  *)
+  Foralltc (fun tc' => node_struct_regular (Zlength lnode) (Znth (Z.of_nat (tc_roottid tc')) lnode)) tc.
+Proof.
+  destruct Hproj as (Hroot & Hproj). hnf in Hroot.
+  apply is_tc_nodearray_proj_regular; auto.
+  - now apply nth_error_some_inrange_Z in Hroot.
+  - apply nth_error_Znth_result in Hroot.
+    hnf. do 4 eexists. rewrite -> Hroot. split; [ reflexivity | ].
+    apply is_tc_nodearray_proj_headch_inrange in Hproj.
+    pose proof (Zlength_nonneg lnode).
+    unfold default_nodefield. intuition lia.
+Qed.
+
+Fact nodearray_proj_regular lnode tc (Hproj1 : is_tc_nodearray_proj_full lnode tc) 
+  (Hproj2 : nodearray_emptypart lnode tc) :
+  (* dim (Hlen : Zlength lnode = dim)  *)
+  Forall (node_struct_regular (Zlength lnode)) lnode.
+Proof.
+  (* revert lnode Hproj1 Hproj2.
+  induction tc as [(u, clk, aclk) chn IH] using treeclock_ind_2; intros. *)
+  apply Forall_Znth.
+  intros n Hr. destruct (tc_getnode (Z.to_nat n) tc) as [ res | ] eqn:E.
+  - apply is_tc_nodearray_proj_full_regular, Foralltc_Forall_subtree in Hproj1.
+    rewrite -> Forall_forall in Hproj1.
+    assert (Datatypes.is_true (ssrbool.isSome (tc_getnode (Z.to_nat n) tc))) as H by now rewrite E.
+    apply tc_getnode_subtc_iff, in_map_iff in H.
+    destruct H as (sub & Eid & Hin). apply Hproj1 in Hin.
+    rewrite -> Eid, -> Z2Nat.id in Hin; auto; try lia.
+  - destruct (nth_error lnode (Z.to_nat n)) eqn:Ee.
+    2:{ apply nth_error_None in Ee. rewrite <- ZtoNat_Zlength in Ee. lia. }
+    pose proof Ee as Ee'.
+    apply nth_error_Znth_result in Ee'. rewrite -> Z2Nat.id in Ee'; auto; try lia.
+    rewrite -> Ee'.
+    apply Hproj2 in Ee; auto. subst.
+    hnf. do 4 eexists. split; [ reflexivity | ].
+    unfold default_nodefield. intuition lia.
+Qed.
 
 Fact is_tc_clockarray_proj_nth lclk tc (Hproj : is_tc_clockarray_proj lclk tc) :
   Foralltc (fun tc' => (Znth (Z.of_nat (tc_roottid tc')) lclk) = 
@@ -221,6 +393,32 @@ Definition join_spec :=
     (* nothing should change for p' *)
     SEP (treeclock_rep dim (tc_join tc tc') plclk plnode plstk top_ p * treeclock_rep dim tc' plclk' plnode' plstk' top' p').
 
+Definition node_is_null_spec :=
+  DECLARE _node_is_null
+  WITH dim : Z, idx : nat, lnode : list (reptype t_struct_node),
+    tc : (@treeclock nat), v1 : val, plnode : val, v2 : val, v3 : val, p : val
+  PRE [ tptr t_struct_node ]
+    PROP (0 <= dim <= Int.max_signed; Z.of_nat idx < dim; 
+      Z.of_nat (tc_roottid tc) < dim; 
+      Zlength lnode = dim; 
+      nodearray_emptypart lnode tc; is_tc_nodearray_proj lnode tc)
+    PARAMS (offset_val (sizeof t_struct_node * Z.of_nat idx) plnode)
+    SEP (data_at Tsh (tarray t_struct_node dim) lnode plnode;
+      data_at Tsh t_struct_treeclock
+        (Vint (Int.repr dim), (Vint (Int.repr (Z.of_nat (tc_roottid tc))), 
+          (v1, (plnode, (v2, v3))))) p)
+  POST [ tint ]
+    PROP () 
+    RETURN (Val.of_bool (
+      (match tc with Node (mkInfo idx' _ _) nil => Nat.eqb idx idx' | _ => false end) ||
+      (match tc_getnode idx tc with None => true | _ => false end)
+    )%bool)
+
+    SEP (data_at Tsh (tarray t_struct_node dim) lnode plnode;
+      data_at Tsh t_struct_treeclock
+        (Vint (Int.repr dim), (Vint (Int.repr (Z.of_nat (tc_roottid tc))), 
+          (v1, (plnode, (v2, v3))))) p).
+
 (*
 
 Section Dim_Bounds.
@@ -236,7 +434,8 @@ Lemma dim_bounds_treeclock_rep_root :
 
 Definition Gprog : funspecs :=
   ltac:(with_library prog [
-    join_spec
+    join_spec; 
+    node_is_null_spec
   ]).
 
 Section Main_Proof.
@@ -251,11 +450,18 @@ Local Tactic Notation "saturate_lemmas" :=
   or make a customized Corollary *)
 
 Local Tactic Notation "array_focus" constr(idx) constr(lstruct) "witheqn" ident(Hy) :=
-  match goal with |- context[data_at Tsh (tarray _ ?size) lstruct _] => 
-    sep_apply (SingletonHole.array_with_hole_intro Tsh _ idx size lstruct); try lia end;
+  (* TODO this part may be extracted to be a compatible generator *)
+  match goal with |- context[data_at Tsh (tarray ?ty ?size) lstruct ?plstruct] => 
+    ((match goal with _ : field_compatible (tarray ty size) [] plstruct |- _ => idtac end) +
+    (let Hcomp := fresh "_Hcomp" in
+      assert_PROP (field_compatible (tarray ty size) [] plstruct) as Hcomp by entailer));
+    sep_apply (SingletonHole.array_with_hole_intro Tsh _ idx size lstruct); try lia 
+  end;
   match goal with |- context[field_address (tarray ?a ?size) (SUB ?b) ?c] => 
     assert (field_address (tarray a size) (SUB b) c = offset_val (sizeof a * b) c) as Hy
-    by (apply arr_field_address; try lia; try assumption) end.
+    by (apply arr_field_address; try lia; try assumption) end; 
+  (* for normalize *)
+  Intros.
 
 Local Tactic Notation "read_clock" "witheqn" hyp(Eclock_payload) :=
   match type of Eclock_payload with 
@@ -272,6 +478,15 @@ Local Tactic Notation "array_unfocus" "witheqn" hyp(Hy) :=
   sep_apply SingletonHole.array_with_hole_elim;
   rewrite upd_Znth_triv; try lia; try reflexivity; clear Hy.
 
+Local Tactic Notation "rewrite_sem_add_ptr_int" :=
+  simpl sem_binary_operation';
+  repeat match goal with |- context[force_val (sem_add_ptr_int ?ty Signed ?p ?v)] => 
+    ((match goal with _ : isptr p |- _ => idtac end) +
+    (let Hisptr := fresh "_Hisptr" in
+      assert_PROP (isptr p) as Hisptr by entailer));
+    rewrite -> sem_add_pi'; auto; try lia
+  end.
+
 (*
 Local Corollary array_with_hole_intro_alt : forall (sh : Share.t) (t : type) (i n : Z) 
     (al : list (reptype t)) (p : val),
@@ -281,6 +496,20 @@ Local Corollary array_with_hole_intro_alt : forall (sh : Share.t) (t : type) (i 
         * SingletonHole.array_with_hole sh t i n al p.
 Proof SingletonHole.array_with_hole_intro.
 *)
+
+Lemma body_node_is_null: 
+  semax_body Vprog Gprog f_node_is_null node_is_null_spec.
+Proof.
+  saturate_lemmas.
+
+  start_function.
+  array_focus (Z.of_nat idx) lnode witheqn Etmp.
+  rewrite -> Etmp.
+
+
+
+  forward.
+Abort.
 
 Theorem body_join: 
   semax_body Vprog Gprog f_join join_spec.
@@ -305,7 +534,6 @@ Proof.
     rewrite -> ! two_power_pos_nat. simpl. lia.
   } *)
 
-  (* pre *) assert_PROP (field_compatible (tarray t_struct_clock dim) [] plclk') as Hcomp by entailer.
   array_focus (Z.of_nat (tc_roottid tc')) lclk' witheqn Etmp.
   (* replacing the following thing *)
   (* 
@@ -322,10 +550,14 @@ Proof.
   (* need compatible *)
   rewrite arr_field_address in Etmp; try lia; try assumption. *)
 
-  simpl.
+  rewrite_sem_add_ptr_int.
+  (*
+  simpl sem_binary_operation'.
   (* pre *) assert_PROP (isptr plclk') as Hip by entailer.
   (* need isptr *)
   rewrite -> sem_add_pi'; auto; try lia.
+  *)
+
   (*
   unfold sem_add_ptr_int.
   replace (complete_type cenv_cs (Tstruct _Clock noattr)) with true by now compute.
@@ -342,7 +574,7 @@ Proof.
   rewrite ptrofs_mul_repr.
   simpl in Etmp.
   *)
-  Intros.
+  (* Intros. *)
   pose proof (Foralltc_self _ _ Hca_tc') as Etmp2. cbn in Etmp2.
   rewrite -> Etmp.
   read_clock witheqn Etmp2. clear Etmp2.
@@ -359,13 +591,18 @@ Proof.
   *)
   array_unfocus witheqn Etmp.
 
-  forward.
-  forward.
-  forward.
-  forward.
-  forward.
+  forward. forward. forward. forward. forward.
+  rewrite_sem_add_ptr_int.
+  (*
+  simpl.
+  (* pre *) assert_PROP (isptr plnode) as Hip0 by entailer.
+  (* pre *) assert_PROP (isptr plclk) as Hip1 by entailer.
+  rewrite -> ! sem_add_pi'; auto; try lia.
+  *)
 
-  deadvars.
+
+
+
 (*
   forward_if (temp _t'1 (Val.of_bool (orb
     (Nat.eqb (tc_roottid tc) (tc_roottid tc'))
