vst/util_vst.v
@@ -1,0 +1,57 @@
+Require Import VST.floyd.proofauto.
+From Coq Require Import List Bool Lia ssrbool PeanoNat Sorting RelationClasses.
+From Coq Require ssreflect.
+Import ssreflect.SsrSyntax.
+
+Section Short_Integer_Type.
+
+Definition short_max_signed := two_power_nat 15 - 1.
+
+(* TODO why so tedious *)
+Fact Zpower_nat_gt_0 b n : b > 0 -> 0 < Zpower_nat b n.
+Proof. induction n; intros; simpl; try nia. Qed.
+
+Fact short_max_signed_le_int_max_signed : short_max_signed <= Int.max_signed.
+Proof. 
+  unfold Int.max_signed, Int.half_modulus, Int.modulus, short_max_signed, Int.wordsize, Wordsize_32.wordsize.
+  unfold two_power_nat. 
+  rewrite -> ! shift_nat_correct, -> ! Z.mul_1_r.
+  rewrite -> Zaux.Zpower_nat_S with (e:=31%nat), -> Z.mul_comm, -> Z_div_mult; try lia.
+  replace 31%nat with (16+15)%nat by lia.
+  rewrite -> Zpower_nat_is_exp.
+  pose proof (Zpower_nat_gt_0 2%Z 15) as H.
+  pose proof (Zpower_nat_gt_0 2%Z 16) as H0. 
+  nia.
+Qed.
+
+Fact short_max_signed_gt_0 : 0 < short_max_signed.
+Proof. 
+  unfold short_max_signed, two_power_nat. 
+  rewrite -> shift_nat_correct, -> Zaux.Zpower_nat_S.
+  pose proof (Zpower_nat_gt_0 2%Z 14) as H. lia.
+Qed.
+
+End Short_Integer_Type.
+
+(* a little fact ... TODO why this is not in stdlib? *)
+Fact nth_error_some_inrange {A : Type} (i : nat) (al : list A) a : 
+  nth_error al i = Some a -> (i < length al)%nat.
+Proof.
+  revert i a. induction al as [ | a' al IH ]; intros; simpl in *.
+  - destruct i; now simpl in H.
+  - destruct i; try lia. simpl in H. apply IH in H. lia.
+Qed.
+
+Fact nth_error_some_inrange_Z {A : Type} (i : nat) (al : list A) a : 
+  nth_error al i = Some a -> Z.of_nat i < Zlength al.
+Proof. 
+  intros H. apply nth_error_some_inrange in H. 
+  rewrite <- ZtoNat_Zlength in H. lia.
+Qed.
+
+Fact nth_error_Znth_result {A : Type} `{Inhabitant A} n (l : list A) res : 
+  nth_error l n = Some res -> Znth (Z.of_nat n) l = res.
+Proof.
+  intros HH. apply List.nth_error_nth with (d:=default) in HH.
+  now rewrite <- nth_Znth'.
+Qed.
